src/sequential/MaxView.v
@@ -319,30 +319,6 @@ Proof.
   { inv FULFILLED. rewrite OTHER in GET2; auto. clarify. eauto. }
 Qed.
 
-Inductive cancel_future_memory (loc: Loc.t) : Memory.t -> Memory.t -> Memory.t -> Memory.t -> Prop :=
-| cancel_future_memory_base
-    prom0 mem0
-  :
-    cancel_future_memory loc prom0 mem0 prom0 mem0
-| cancel_future_memory_step
-    prom0 mem0 prom1 mem1 prom2 mem2
-    from to
-    (CANCEL: Memory.promise prom0 mem0 loc from to Message.reserve prom1 mem1 Memory.op_kind_cancel)
-    (FUTURE: cancel_future_memory loc prom1 mem1 prom2 mem2)
-  :
-    cancel_future_memory loc prom0 mem0 prom2 mem2
-.
-
-Lemma cancel_future_reserve_future loc prom0 mem0 prom1 mem1
-      (CANCEL: cancel_future_memory loc prom0 mem0 prom1 mem1)
-  :
-    reserve_future_memory prom0 mem0 prom1 mem1.
-Proof.
-  induction CANCEL; eauto.
-  { econs 1; eauto. }
-  { econs 2; eauto. }
-Qed.
-
 Variant unchanged_loc_memory (loc: Loc.t) (mem0 mem1: Memory.t): Prop :=
 | unchanged_loc_memory_intro
     (UNCH: forall to, Memory.get loc to mem1 = Memory.get loc to mem0)
